\documentclass{article}
\usepackage{amsmath,amssymb,amsthm,latexsym,paralist,url}
\usepackage[margin=1in]{geometry}
\usepackage{tikz}
\usetikzlibrary{arrows,automata}
\usepackage{csquotes}
\usepackage[ruled]{algorithm2e}

\theoremstyle{definition}
\newtheorem*{problem}{Problem}
\newtheorem*{solution}{Solution}



\begin{document}


% Chapter 4.1, Problem 14
\begin{problem}[Rosen.4.1.14]\ \\
Prove that for every positive integer n, $\displaystyle \sum_{i=1}^n i*2^i = (n-1)*2^{n+1}+2$.
\end{problem}

\begin{solution}\ \\
{\color{red}
\noindent
Let $P(n):=$ $\sum_{i=1}^{n} 2^{i} i = 2^{n + 1} \left(n - 1\right) + 2$, when $n\geq 1$\\
\\
\textbf{Basis Step:} $P(1)$ \\

$\sum_{i=1}^{1} 2^{i} i = 2$\\

$2^{1 + 1} \left(1 - 1\right) + 2 = 2$\\

$\therefore  P(1)$ holds.\\
\\
\textbf{Inductive Step:} $P(k)\implies P(k+1)$\\

Assume $P(k)$ for some $k\geq 1:$ $\sum_{i=1}^{k} 2^{i} i = 2^{k + 1} \left(k - 1\right) + 2$\\

Show $P(k+1):$ $\sum_{i=1}^{k + 1} 2^{i} i = 2^{k + 2} k + 2$\\

$\sum_{i=1}^{k + 1} 2^{i} i = 2^{k + 1} \left(k + 1\right) + \sum_{i=1}^{k} 2^{i} i$\\

$ = 2^{k + 1} \left(k - 1\right) + 2^{k + 1} \left(k + 1\right) + 2$  \hfill (by inductive hypothesis)\\

$ = 2 \cdot 2^{k+1} k + 2 = 2^{k + 2} k + 2$\\

$\therefore  P(k)\implies P(k+1)$ holds for $k \geq 1$.\\

\noindent
$\therefore P(n)$ holds for all $n \geq 1$ by mathematical induction. \qed
}
\end{solution}

\end{document}
