\documentclass{article}
\usepackage{amsmath,amssymb,amsthm,latexsym,paralist,url}
\usepackage[margin=1in]{geometry}
\usepackage{tikz}
\usetikzlibrary{arrows,automata}
\usepackage{csquotes}
\usepackage[ruled]{algorithm2e}

\theoremstyle{definition}
\newtheorem*{problem}{Problem}
\newtheorem*{solution}{Solution}



\begin{document}


% Chapter 5.1, Problem 25
\begin{problem}[Rosen.5.1.25]\ \\
Prove by mathematical induction on $n$ that if $h > -1$, then $1+nh \leq (1+h)^n$ for all nonnegative integers $n$.  This is called \textbf{Bernoulli's inequality}.
\end{problem}

\begin{solution}\ \\
{\color{red}
$P(n) := $ if $h > -1$, then $1+nh \leq (1+h)^n$\\
\\
\textbf{Basis Step:} $P(0)$

Let $h > -1$.

$1 + nh = 1 + (0)h = 1$

$(1+h)^0 = 1$

$1=1$ \checkmark

$\therefore P(0)$ holds.\\
\\
\textbf{Inductive Step:} $P(k) \to P(k+1)$

Assume $P(k)$ for some $k \geq 0$: if $h > -1$, then $1+kh \leq (1+h)^k$.

Show $P(k+1):$ if $h > -1$, then $1+(k+1)h \leq (1+h)^{k+1}$

Let $h > -1$.

(Started on LHS, got stuck.  Trying again from RHS)

$(1+h)^{k+1}$

$= (1+h)^k(1+h)$

$\geq (1+kh)(1+h)$ by inductive hypothesis

$= 1 + h + kh + kh^2$

$= 1 + (k+1)h + kh^2$

$\geq 1 + (k+1)h$ since $k \geq 0$ \checkmark

$\therefore P(k) \to P(k+1)$ holds.\\
\\
$\therefore P(n)$ holds for all $n \geq 0$ by PMI. \qed
}
\end{solution}

\end{document}
